Show basic results for mappings over lists

ProofLibrary/Models/Cores.lean
@@ -1,45 +1,244 @@
 import ProofLibrary.SubstitutionAndHomomorphismBasics
 
+namespace List
+
+  theorem length_le_of_nodup_of_all_mem [DecidableEq α] (as bs : List α) (nodup : as.Nodup) (all_mem : ∀ e, e ∈ as -> e ∈ bs) : as.length ≤ bs.length := by
+    induction as generalizing bs with
+    | nil => simp
+    | cons a as ih =>
+      let bs_without_a := bs.erase a
+      simp at nodup
+      specialize ih
+        bs_without_a
+        nodup.right
+        (by intro c c_mem; rw [List.mem_erase_of_ne]; apply all_mem; simp [c_mem]; intro contra; rw [contra] at c_mem; apply nodup.left; exact c_mem)
+      rw [List.length_erase_of_mem (by apply all_mem; simp)] at ih
+      rw [Nat.le_sub_one_iff_lt (by apply List.length_pos_of_mem; apply all_mem a; simp)] at ih
+      apply Nat.succ_le_of_lt
+      exact ih
+
+  theorem equiv_of_nodup_of_length_eq_of_all_mem [DecidableEq α] (as bs : List α) (nodup : as.Nodup) (eq_length : as.length = bs.length) (all_mem : ∀ e, e ∈ as -> e ∈ bs) : ∀ e, e ∈ as ↔ e ∈ bs := by
+    intro e
+    constructor
+    . apply all_mem
+    . intro mem_bs
+      induction as generalizing bs e with
+      | nil => cases bs; simp at mem_bs; simp at eq_length
+      | cons a as ih =>
+        let bs_without_a := bs.erase a
+        simp at nodup
+        specialize ih
+          bs_without_a
+          nodup.right
+          (by rw [List.length_erase_of_mem, ← eq_length]; simp; apply all_mem; simp)
+          (by intro c c_mem; rw [List.mem_erase_of_ne]; apply all_mem; simp [c_mem]; intro contra; rw [contra] at c_mem; apply nodup.left; exact c_mem)
+        cases Decidable.em (e = a) with
+        | inl eq => simp [eq]
+        | inr neq =>
+          simp; apply Or.inr
+          apply ih
+          rw [List.mem_erase_of_ne]
+          exact mem_bs
+          exact neq
+end List
+
 namespace Function
 
-  def injective (f : α -> β) : Prop := ∀ a b, f a = f b -> a = b
+  def injective_for_domain_set (f : α -> β) (domain : Set α) : Prop := ∀ a a', a ∈ domain -> a' ∈ domain -> f a = f a' -> a = a'
+  def surjective_for_domain_and_image_set (f : α -> β) (domain : Set α) (image : Set β) : Prop := ∀ b, b ∈ image -> ∃ a, a ∈ domain ∧ f a = b
 
-  def surjective (f : α -> β) : Prop := ∀ b, ∃ a, f a = b
+  def injective_for_domain_list (f : α -> β) (domain : List α) : Prop := ∀ a a', a ∈ domain -> a' ∈ domain -> f a = f a' -> a = a'
+  def surjective_for_domain_and_image_list (f : α -> β) (domain : List α) (image : List β) : Prop := ∀ b, b ∈ image -> ∃ a, a ∈ domain ∧ f a = b
+
+  theorem injective_set_list_equiv (f : α -> β) (domain_set : Set α) (domain_list : List α) (eq : ∀ e, e ∈ domain_list ↔ e ∈ domain_set) : f.injective_for_domain_set domain_set ↔ f.injective_for_domain_list domain_list := by
+    constructor
+    . intro h a a' a_mem a'_mem f_eq
+      apply h
+      . rw [← eq]; assumption
+      . rw [← eq]; assumption
+      . exact f_eq
+    . intro h a a' a_mem a'_mem f_eq
+      apply h
+      . rw [eq]; assumption
+      . rw [eq]; assumption
+      . exact f_eq
+
+  theorem surjective_set_list_equiv (f : α -> β)
+      (domain_set : Set α) (domain_list : List α) (eq_domain : ∀ e, e ∈ domain_list ↔ e ∈ domain_set)
+      (image_set : Set β) (image_list : List β) (eq_image : ∀ e, e ∈ image_list ↔ e ∈ image_set) :
+      f.surjective_for_domain_and_image_set domain_set image_set ↔ f.surjective_for_domain_and_image_list domain_list image_list := by
+    constructor
+    . intro h b b_mem
+      specialize h b (by rw [← eq_image]; exact b_mem)
+      rcases h with ⟨a, a_mem, a_eq⟩
+      exists a
+      constructor
+      . rw [eq_domain]; exact a_mem
+      . exact a_eq
+    . intro h b b_mem
+      specialize h b (by rw [eq_image]; exact b_mem)
+      rcases h with ⟨a, a_mem, a_eq⟩
+      exists a
+      constructor
+      . rw [← eq_domain]; exact a_mem
+      . exact a_eq
+
+  theorem injective_for_domain_list_cons (f : α -> β) (hd : α) (tl : List α) : f.injective_for_domain_list (hd::tl) -> f.injective_for_domain_list tl := by
+    intro h a a' a_mem a'_mem eq
+    apply h
+    . simp [a_mem]
+    . simp [a'_mem]
+    . exact eq
+
+  def image [DecidableEq β] (f : α -> β) : List α -> List β
+  | [] => []
+  | hd::tl =>
+    let tl_img := image f tl
+    if f hd ∈ tl_img then tl_img else (f hd)::tl_img
+
+  theorem mapping_mem_image_of_mem [DecidableEq β] (f : α -> β) (domain : List α) : ∀ a, a ∈ domain -> f a ∈ (image f domain) := by
+    intro a a_mem
+    induction domain with
+    | nil => simp at a_mem
+    | cons hd tl ih =>
+      simp [image]
+      cases Decidable.em (f hd ∈ image f tl) with
+      | inl hd_mem => simp [image, hd_mem]; cases a_mem; exact hd_mem; apply ih; assumption
+      | inr hd_not_mem => simp [image, hd_not_mem]; cases a_mem; apply Or.inl; rfl; apply Or.inr; apply ih; assumption
+
+  theorem nodup_image [DecidableEq β] (f : α -> β) (domain : List α) : (image f domain).Nodup := by
+    induction domain with
+    | nil => simp [image]
+    | cons hd tl ih =>
+      cases Decidable.em (f hd ∈ image f tl) with
+      | inl hd_mem => simp [image, hd_mem]; exact ih
+      | inr hd_not_mem => simp [image, hd_not_mem]; exact ih
+
+  theorem length_image [DecidableEq β] (f : α -> β) (domain : List α) : (image f domain).length ≤ domain.length := by
+    induction domain with
+    | nil => simp [image]
+    | cons hd tl ih => simp [image]; split; apply Nat.le_trans; exact ih; simp; simp; exact ih
+
+  theorem surjective_on_own_image [DecidableEq β] (f : α -> β) (domain : List α) : f.surjective_for_domain_and_image_list domain (image f domain) := by
+    induction domain with
+    | nil => simp [surjective_for_domain_and_image_list, image]
+    | cons hd tl ih =>
+      intro b b_mem
+      cases Decidable.em (f hd ∈ image f tl) with
+      | inl hd_mem => simp [image, hd_mem] at b_mem; rcases ih b b_mem with ⟨a, ha⟩; exists a; simp [ha]
+      | inr hd_not_mem =>
+        simp [image, hd_not_mem] at b_mem
+        cases b_mem with
+        | inr b_mem => rcases ih b b_mem with ⟨a, ha⟩; exists a; simp [ha]
+        | inl b_mem => exists hd; simp [b_mem]
+
+  theorem image_contained_of_closed [DecidableEq α] (f : α -> α) (domain : List α) (closed : ∀ e, e ∈ domain -> f e ∈ domain) : ∀ e, e ∈ image f domain -> e ∈ domain := by
+    intro b b_mem
+    rcases surjective_on_own_image f domain b b_mem with ⟨a, a_mem, a_eq⟩
+    rw [← a_eq]
+    apply closed
+    exact a_mem
+
+  theorem injective_iff_length_image_eq_of_nodup [DecidableEq β] (f : α -> β) (domain : List α) (nodup : domain.Nodup) : f.injective_for_domain_list domain ↔ (image f domain).length = domain.length := by
+    constructor
+    . intro inj
+      induction domain with
+      | nil => simp [image]
+      | cons hd tl ih =>
+        cases Decidable.em (f hd ∈ image f tl) with
+        | inl hd_mem =>
+          apply False.elim
+          simp at nodup
+          apply nodup.left
+          rcases surjective_on_own_image f tl (f hd) hd_mem with ⟨a, a_mem, a_eq⟩
+          specialize inj a hd (by simp [a_mem]) (by simp) a_eq
+          rw [← inj]
+          exact a_mem
+        | inr hd_not_mem =>
+          simp [image, hd_not_mem]
+          apply ih
+          . simp at nodup; exact nodup.right
+          . apply injective_for_domain_list_cons; exact inj
+    . intro length_eq
+      induction domain with
+      | nil => simp [injective_for_domain_list]
+      | cons hd tl ih =>
+        cases Decidable.em (f hd ∈ image f tl) with
+        | inl hd_mem =>
+          simp [image, hd_mem] at length_eq
+          have contra := length_image f tl
+          rw [length_eq] at contra
+          simp [Nat.succ_le] at contra
+        | inr hd_not_mem =>
+          simp [image, hd_not_mem] at length_eq
+          intro a a' a_mem a'_mem eq
+          cases a_mem
+          . cases a'_mem
+            . rfl
+            . apply False.elim
+              apply hd_not_mem
+              rw [eq]
+              apply mapping_mem_image_of_mem
+              assumption
+          . cases a'_mem
+            . apply False.elim
+              apply hd_not_mem
+              rw [← eq]
+              apply mapping_mem_image_of_mem
+              assumption
+            . simp at nodup
+              specialize ih nodup.right length_eq
+              apply ih <;> assumption
+
+  theorem surjective_on_target_iff_all_in_image [DecidableEq β] (f : α -> β) (domain : List α) (target_image : List β) : f.surjective_for_domain_and_image_list domain target_image ↔ ∀ b, b ∈ target_image -> b ∈ image f domain := by
+    constructor
+    . intro surj b b_mem
+      specialize surj b b_mem
+      rcases surj with ⟨a, a_mem, a_eq⟩
+      rw [← a_eq]
+      apply mapping_mem_image_of_mem
+      exact a_mem
+    . intro h b b_mem
+      apply surjective_on_own_image
+      apply h
+      exact b_mem
+
+  theorem injective_iff_surjective_of_nodup_of_closed [DecidableEq α] (f : α -> α) (l : List α) (nodup : l.Nodup) (closed : ∀ e, e ∈ l -> f e ∈ l) : f.injective_for_domain_list l ↔ f.surjective_for_domain_and_image_list l l := by
+    constructor
+    . intro inj
+
+      have : ∀ e, e ∈ image f l ↔ e ∈ l := by
+        apply List.equiv_of_nodup_of_length_eq_of_all_mem
+        . apply nodup_image
+        . rw [injective_iff_length_image_eq_of_nodup] at inj
+          rw [inj]
+          exact nodup
+        . intro e e_mem
+          apply image_contained_of_closed
+          . exact closed
+          . exact e_mem
+
+      rw [surjective_on_target_iff_all_in_image]
+      intro b
+      apply (this b).mpr
+    . intro surj
+      rw [surjective_on_target_iff_all_in_image] at surj
+      rw [injective_iff_length_image_eq_of_nodup _ _ nodup]
+      rw [Nat.eq_iff_le_and_ge]
+      constructor
+      . exact length_image f l
+      . exact List.length_le_of_nodup_of_all_mem l (image f l) nodup surj
 
 end Function
+
+
 
 namespace GroundTermMapping
 
   variable {sig : Signature} [DecidableEq sig.P] [DecidableEq sig.C] [DecidableEq sig.V]
 
-  -- TODO: do we really need this?
-  def injective (h : GroundTermMapping sig) (terms : Set (GroundTerm sig)) : Prop :=
-    ∀ t t', (t ∈ terms ∧ t' ∈ terms) -> (h t = h t' -> t = t')
-
-  -- TODO: do we really need this?
-  def surjective (h : GroundTermMapping sig) (terms : Set (GroundTerm sig)) : Prop :=
-    ∀ t', t' ∈ terms -> ∃ t, h t = t'
-
   def strong (h : GroundTermMapping sig) (A B : FactSet sig) : Prop :=
     ∀ e, ¬ e ∈ A -> ¬ (h.applyFact e) ∈ B
-
-  -- TODO: is this really usable?
-  theorem surjective_of_injective_of_closed_on_list (h : GroundTermMapping sig) (terms : List (GroundTerm sig)) (inj : h.injective terms.toSet) (closed : ∀ (l : List _), ∀ t, t ∈ l -> h t ∈ l) : h.surjective terms.toSet := by
-    induction terms with
-    | nil => sorry
-    | cons hd tl ih =>
-      specialize ih (sorry)
-      unfold surjective
-      intro b b_mem
-      rw [← List.inIffInToSet] at b_mem
-      simp at b_mem
-      cases b_mem with
-      | inl b_mem => sorry
-      | inr b_mem =>
-        unfold surjective at ih
-        rw [List.inIffInToSet] at b_mem
-        specialize ih b b_mem
-        exact ih
 
 end GroundTermMapping
 
@@ -48,10 +247,10 @@ namespace FactSet
   variable {sig : Signature} [DecidableEq sig.P] [DecidableEq sig.C] [DecidableEq sig.V]
 
   def isWeakCore (fs : FactSet sig) : Prop :=
-    ∀ (h : GroundTermMapping sig), h.isHomomorphism fs fs -> h.strong fs fs ∧ h.injective fs.terms
+    ∀ (h : GroundTermMapping sig), h.isHomomorphism fs fs -> h.strong fs fs ∧ h.injective_for_domain_set fs.terms
 
   def isStrongCore (fs : FactSet sig) : Prop :=
-    ∀ (h : GroundTermMapping sig), h.isHomomorphism fs fs -> h.strong fs fs ∧ h.injective fs.terms ∧ h.surjective fs.terms
+    ∀ (h : GroundTermMapping sig), h.isHomomorphism fs fs -> h.strong fs fs ∧ h.injective_for_domain_set fs.terms ∧ h.surjective_for_domain_and_image_set fs.terms fs.terms
 
   theorem isStrongCore_of_isWeakCore_of_finite (fs : FactSet sig) (weakCore : fs.isWeakCore) (finite : fs.finite) : fs.isStrongCore := by
     rcases finite with ⟨l, finite⟩
@@ -63,8 +262,11 @@ namespace FactSet
     . exact strong
     constructor
     . exact injective
-    . intro b b_mem
-      sorry
+    . let terms_list := (l.map Fact.terms).flatten -- TODO: maybe dedup needed...
+      rw [Function.surjective_set_list_equiv h fs.terms terms_list sorry fs.terms terms_list sorry]
+      rw [← Function.injective_iff_surjective_of_nodup_of_closed h terms_list sorry sorry]
+      rw [← Function.injective_set_list_equiv h fs.terms terms_list sorry]
+      exact injective
 
 end FactSet
 
